Dummy instruction level

compiler.v
@@ -1,4 +1,5 @@
 Require Import Coq.ZArith.BinInt.
+Require Import Coq.Lists.List. Import ListNotations.
 Require Import PeanoNat.
 
 (* Option monad utilities *)
@@ -16,7 +17,7 @@ Definition Regs := nat -> Z.
 
 Fixpoint get (var : Var) (r : Regs) := r var.
 
-Fixpoint put (r : Regs) (var : Var) v :=
+Fixpoint put (var : Var) v (r : Regs) :=
   fun var' => if var' =? var then v else r var'.
 
 (* Registers are zeroed by default *)
@@ -37,7 +38,7 @@ Fixpoint eval_stmt_log (s : Stmt) (fuel : nat) (r : Regs) :=
   match fuel with
   | O => None
   | S f => match s with
-           | SAdd a b c => Some (1%Z, put r a ((get b r) + (get c r)))
+           | SAdd a b c => Some (1%Z, put a ((get b r) + (get c r)) r)
            | SIf cond trueEval falseEval => if (Z.eqb (get cond r) 0%Z) then
                                               inc_eval_log (eval_stmt_log falseEval f r) 1%Z
                                             else
@@ -46,22 +47,74 @@ Fixpoint eval_stmt_log (s : Stmt) (fuel : nat) (r : Regs) :=
                            | None => None
                            | Some (count, r') => inc_eval_log (eval_stmt_log s2 f r') count
                            end
-           | SLit a v => Some (1%Z, put r a v)
+           | SLit a v => Some (1%Z, put a v r)
            end
   end.
 
 Definition var_1 := 1.
 Definition var_a := 2.
 
-(* Test stmt, loads 5 into var_a and doubles it *)
-Definition eg_double_stmt :=
-  SSeq (SLit var_a 5%Z) (SAdd var_a var_a var_a).
+(* Test stmt, loads n into var_a and doubles it *)
+Definition eg_double_stmt n :=
+  SSeq (SLit var_a n) (SAdd var_a var_a var_a).
 
-Definition eg_double_res := (eval_stmt_log eg_double_stmt 5 emptyRegs).
+Definition eg_double_res n := (eval_stmt_log (eg_double_stmt n) 5 emptyRegs).
 
-Definition eg_double_instructions := bind eg_double_res fst.
-Definition eg_double_regs := bind eg_double_res snd.
-Definition eg_double_val := bind eg_double_regs (get var_a).
+Definition eg_double_instructions n := bind (eg_double_res n) fst.
+Definition eg_double_regs n := bind (eg_double_res n) snd.
+Definition eg_double_val n := bind (eg_double_regs n) (get var_a).
 
-Lemma eg_double_val_correct : eg_double_val = Some 10%Z.
+Lemma eg_double_5_correct : eg_double_val 5%Z = Some 10%Z.
 Proof. reflexivity. Qed.
+
+Lemma eg_double_neg12_correct : eg_double_val (Z.neg 12) = Some (Z.neg 24).
+Proof. reflexivity. Qed.
+
+Inductive Instr :=
+  | IAdd (a b c : Var)
+  | IJump (pc : nat) 
+  | IBeqz (a : Var) (pc : nat)
+  | IImm (a : Var) (v : Z)
+  .
+
+Fixpoint compile_stmt (s : Stmt) :=
+  match s with
+  | SAdd a b c => [IAdd a b c]
+  | SIf c t f => match (compile_stmt t) with
+                 | t' => match (compile_stmt f) with
+                         | f' => [IBeqz c (length t')] ++ t' ++ [IJump (length f')] ++ f'
+                         end
+                 end
+  | SSeq s1 s2 => (compile_stmt s1) ++ (compile_stmt s2)
+  | SLit a v => [IImm a v]
+  end.
+
+Fixpoint eval_instr_log_single i regs pc :=
+  match i with
+  | IAdd a b c => (1%Z, put a ((get b regs) + (get c regs)) regs, pc + 1)
+  | IJump pc' => (1%Z, regs, pc')
+  | IBeqz a pc' => (1%Z, regs, if (Z.eqb (get a regs) 0%Z) then pc' else pc + 1)
+  | IImm a v => (1%Z, put a v regs, pc + 1)
+  end.
+
+Fixpoint eval_instr_log (instrs : list Instr) fuel regs pc :=
+  match fuel with
+  | 0 => None
+  | S f => match nth_error instrs pc with
+           | None => Some (0%Z, regs, pc) (* Execution has completed *)
+           | Some i => match (eval_instr_log_single i regs pc) with
+                       | (count', regs', pc') => match (eval_instr_log instrs f regs' pc') with
+                                               | None => None
+                                               | Some (count'', regs'', pc'') => Some (Z.add count' count'', regs'', pc'')
+                                               end
+                       end
+           end 
+  end.
+
+Definition get_compiled_result (s: Stmt) (result_var : Var) :=
+  match eval_instr_log (compile_stmt s) 100 emptyRegs 0 with
+  | None => None
+  | Some (count, regs, pc) => Some (get result_var regs)
+  end.
+
+Compute get_compiled_result (eg_double_stmt 7) var_a.
